Lots of fun extensions to reification

Reify.v
@@ -2,85 +2,226 @@
 Module Reify.
 Require Import Infrastructure.
 Import Infrastructure.
-  Inductive ReiType :=
+
+(* Constructs stolen from Infrastructure.v *)
+Inductive phantom {T : Type} (t : T) : Type := Phantom.
+Definition unify {T1 T2} (t1 : T1) (t2 : T2) :=
+  phantom t1 -> phantom t2.
+
+Structure unify2 {T1 T2} (t1 : T1) (t2 : T2) :=
+  Unify2 {f : phantom t1 -> phantom t2}.
+
+Definition id {T : Type} {t : T} (x : phantom t) := x.    
+
+Canonical Structure unify2_id {T1 : Type} (t1 : T1) :=
+  @Unify2 T1 T1 t1 t1 id.      
+
+(*Canonical Structure unif_id_nat (T : Type) : @unify T T  :=
+    @Unify T T (@id T).*)
+
+
+Inductive ReiType :=
+(* primitive set *)
 | RNat
 | RBool
 | RUnit
-| RPair : ReiType -> ReiType -> ReiType.
+(* primitive type *)
+| RType
+| RSet
+| RProp
+(* combinators *)
+| RPair : ReiType -> ReiType -> ReiType
+| RFunc : ReiType -> ReiType -> ReiType.
 
-  Fixpoint denote (R : ReiType) : Type :=
+Fixpoint denote (R : ReiType) : Type :=
     match R with
       | RNat => nat
       | RBool => bool
       | RUnit => unit
+      | RType => Type
+      | RSet => Set
+      | RProp => Prop
       | RPair i1 i2 => prod (denote i1) (denote i2)
+      | RFunc i1 i2 => ((denote i1) -> (denote i2))
     end.
 
-  Structure tagged_ReiType := RTag {runtag :> ReiType}.
-
+  (*Structure tagged_ReiType := RTag {runtag :> ReiType}.
+*)
+(*
   Structure reifiable :=
     Reifiable {sort : Type;
                rt_of :> tagged_ReiType;
                _ : sort = denote rt_of}.
+*)
+
+  Structure reifiable :=
+    Reifiable {sort : Type;
+               rt_of :> ReiType;
+               _ : sort = denote rt_of}.
+
+  Structure reified :=
+    Reified { T : Type;
+              t : T;
+              rbl_of :> reifiable;
+              _ : T = sort rbl_of}.
+
+  (* no args implicit, will mostly be called from
+     notations in any case *)
+
   
-  Definition nat_tag R := RTag R.
+
+  (*
+  Definition reify_term {T : Type} {rei : reifiable} (t : T)
+             (uni : unify t ()) : .
+   *)
+
+  (*
+  Definition Type_tag R := RTag R.
+  Definition Set_tag R := Type_tag R.
+  Definition Prop_tag R := Set_tag R.
+  Definition nat_tag R := Prop_tag R.
   Definition bool_tag R := nat_tag R.
   Definition unit_tag R := bool_tag R.
   Canonical Structure pair_tag R := unit_tag R.
+   *)
 
-  Canonical Structure rei_nat : reifiable :=
-    Reifiable nat (nat_tag RNat) (eq_refl).
+  Canonical Structure rbl_nat : reifiable :=
+    Reifiable nat RNat eq_refl.
 
-  Canonical Structure rei_bool : reifiable :=
-    Reifiable bool (bool_tag RBool) (eq_refl).
+  (* bool and instances *)
+  Canonical Structure rbl_bool : reifiable :=
+    Reifiable bool RBool eq_refl.
 
-  Canonical Structure rei_unit : reifiable  :=
-    Reifiable unit (unit_tag RUnit) (eq_refl).
+  Canonical Structure rbl_type : reifiable :=
+    Reifiable Type RType eq_refl.
 
-  Lemma rei_pair_proof : forall (r1 r2: reifiable),
+  Canonical Structure rbl_set : reifiable :=
+    Reifiable Set RSet eq_refl.
+
+  Canonical Structure rprop_set : reifiable :=
+    Reifiable Prop RProp eq_refl.
+  
+(*
+  Canonical Structure rfd_true : reified :=
+    @Reified _ _ true eq_refl.
+
+  Canonical Structure rfd_false : reified :=
+    @Reified _ _ false eq_refl.
+*)
+
+  (* should this be rbl or _ ?*)
+  Definition reify_term {T : Type} (t : T) {rbl : reifiable}
+             (eq : T = (sort rbl)) : reified :=
+    Reified T t rbl eq.
+
+  
+  Eval compute in (reify_term True eq_refl).
+
+  Eval compute in (reify_term Type eq_refl).
+
+  (* do we need one or both levels of search *)
+  (* outer eq_refl triggers unification between term at T.
+     we want that to be guaranteed immediately, so we fill it in now
+     inner eq_refl is the one we care about, it is a commitment
+     to a particular reified representation *)
+
+  (* Reify a term, forcing its type *)
+  Notation "{| term :~ T |}" :=
+    (Reified T term _ eq_refl) (at level 60).
+
+  (* Reify a term, a force its type to whatever
+     Coq currently thinks the type is *)
+  Notation "{{| term |}}" :=
+    (Reified _ term _ eq_refl).
+
+  (*  Reify a term, but do not force its type *)
+  Notation "{{ term }}" :=
+    (fun equ =>
+       (Reified _ term _ equ)) (at level 59).
+
+  (* I need to think about this more
+     What I'd really like to have is a more uniform way of
+     talking about unification goals - maybe have a monad of
+     unification contexts? *)
+
+  (* Notations for displaying ReiTypes *)  
+
+  Canonical Structure rbl_unit : reifiable  :=
+    Reifiable unit RUnit eq_refl.
+
+  Lemma rbl_func_proof : forall (dom cod : reifiable),
+                           (sort dom -> sort cod) = denote (RFunc dom cod).
+    Proof.
+      intros.
+      dependent inversion dom. subst. simpl.
+      dependent inversion cod. subst. simpl.
+      reflexivity.
+    Qed.
+
+  Canonical Structure rbl_func (dom cod : reifiable) : reifiable :=
+    Reifiable (sort dom -> sort cod) (RFunc dom cod) (rbl_func_proof dom cod).    
+
+  Lemma rbl_pair_proof : forall (r1 r2: reifiable),
                            prod (sort r1) (sort r2) = denote (RPair r1 r2).
     dependent inversion r1. subst. simpl.
     dependent inversion r2. subst. simpl.
     reflexivity.
   Qed.
 
-  Canonical Structure rei_pair (r1 r2 : reifiable) : reifiable :=
+  Canonical Structure rbl_pair (r1 r2 : reifiable) : reifiable :=
     Reifiable (prod (sort r1) (sort r2))
-              (pair_tag (RPair (rt_of r1) (rt_of r2)))
-              (rei_pair_proof r1 r2).
+              (RPair (rt_of r1) (rt_of r2))
+              (rbl_pair_proof r1 r2).
+
+
+  Eval compute in (rt_of {{| fun (n : nat) m => m n + 1 |}}).
+
+  (* show RFunc RNat (RFunc (RFunc RNat RNat) RNat
+     as <<nat -> nat -> nat>>
+     *)
+
+(*
+  type is a Type (that we want to display)
+  RT is a reified type
+*)
 
   (* concept of "matching" *)
+  (* don't think we need this *)
   Definition check_type
              {reT : reifiable} (t : sort reT):=
     rt_of reT.
 
   Eval compute in (check_type (true, (1, tt))).
 
-  (* Constructs stolen from Infrastructure.v *)
-  Inductive phantom {T : Type} (t : T) : Type := Phantom.
-  Definition unify {T1 T2} (t1 : T1) (t2 : T2) :=
-    phantom t1 -> phantom t2.
+  Eval simpl in (rt_of {{| (fun q : nat => q)  |}}).
 
-  Structure unify2 {T1 T2} (t1 : T1) (t2 : T2) :=
-    Unify2 {f : phantom t1 -> phantom t2}.
-
-  Definition id {T : Type} {t : T} (x : phantom t) := x.    
-
-  Canonical Structure unify2_id {T1 : Type} (t1 : T1) :=
-    @Unify2 T1 T1 t1 t1 id.      
-
-  (*Canonical Structure unif_id_nat (T : Type) : @unify T T  :=
-    @Unify T T (@id T).*)
-
-  Check unify2.
-  Check unify2_id.
+  Eval compute in (T {{|3|}}).
 
   Definition get_type {reT : reifiable} (T : Type) (uni : unify T (sort reT)) :=
-    rt_of reT.
+    reT.
+
+  Check @get_type.
+
+  Print reifiable.
+
+  Definition tylift' (T : Type) {rbl : reifiable}
+             (uni : denote (rt_of rbl) = T):= 
+    rt_of rbl.
+
+
+  Check rt_of.
+
+  Eval simpl in (rt_of {{| fun (n : nat) m => m n + 1 |}}).
+
 
   Notation "f ! x" := (f x id) (at level 99).
 
-  Eval compute in (get_type! nat).
+  Eval compute in (get_type! (nat * (bool * unit)%type)%type).
+
+  Canonical Structure rei_Type :
+
+  Canonical Structure rei_Type {T : Type} {reT : reifiable} (uni : unify T (sort re
+
 
   Definition get_type {reT : reifiable} (T : Type) : ReiType :=
     get_type' T id.
@@ -179,4 +320,4 @@ Require Import Infrastructure.
   Eval compute in (get_type (false, (true, false))).
 
 End Reify.
-n
+
